

Tutorial 2

LTI Systems

Linear Systems

① Homogeneity $x(t) \rightarrow \boxed{} \rightarrow y(t) \Rightarrow a x(t) \rightarrow \boxed{} \rightarrow a y(t)$

② Additivity/ Superposition $\left. \begin{array}{l} x_1(t) \rightarrow \boxed{} \rightarrow y_1(t) \\ x_2(t) \rightarrow \boxed{} \rightarrow y_2(t) \end{array} \right\} \Rightarrow x_1(t) + x_2(t) \rightarrow \boxed{} \rightarrow y_1(t) + y_2(t)$

If ① and ② hold, the system is **linear**

$$a_n(x) \frac{d^n y(t)}{dt^n} + a_{n-1}(x) \frac{d^{n-1} y(t)}{dt^{n-1}} + \dots + a_1(x) \frac{dy(t)}{dt} + a_0(x) y(t) = b(x)$$

describes a general linear differential equation

Time Invariance

defn: A system is **time-invariant** if it is described by differential equations and all the coefficients are constant wrt time

$$\begin{array}{l} x(t) \rightarrow \boxed{} \rightarrow y(t) \\ x(t-t_0) \rightarrow \boxed{} \rightarrow y(t, t_0) \stackrel{?}{=} y(t-t_0) \end{array} \rightarrow \begin{array}{l} \text{yes} \Rightarrow \text{time invariant} \\ \text{no} \Rightarrow \text{time varying} \end{array}$$

highlight time shifted input

Example 2.1

a. $y(t) = 2t^2 x(t)$ *time shifted input*
 $y(t, t_0) = 2t^2 x(t-t_0)$
 $y(t-t_0) = 2(t-t_0)^2 x(t-t_0)$ $\left. \begin{array}{l} y(t, t_0) \neq y(t-t_0) \end{array} \right\} \Rightarrow \text{time varying}$

$$\begin{array}{l} a y(t) = 2t^2 a x(t) \\ y_1(t) = 2t^2 x_1(t) \\ y_2(t) = 2t^2 x_2(t) \end{array} \left. \begin{array}{l} y_1(t) + y_2(t) = 2t^2 (x_1(t) + x_2(t)) \end{array} \right\} \text{linear}$$

b. $y(t) = 3e^{3x(t)}$
 $y(t, t_0) = 3e^{3x(t-t_0)}$
 $y(t-t_0) = 3e^{3x(t-t_0)}$ $\left. \begin{array}{l} y(t, t_0) = y(t-t_0) \end{array} \right\} \Rightarrow \text{time invariant}$

$$3a e^{3x(t)} \neq 3e^{3ax(t)} \Rightarrow \text{violates homogeneity} \Rightarrow \text{easy way to tell: } \begin{cases} \text{if } a < 0 \\ 3a e^{3x(t)} < 0 \\ 3e^{3ax(t)} > 0 \end{cases}$$

$\Rightarrow \text{nonlinear}$

c. $5t^2 \frac{d^2 y(t)}{dt^2} + 4y(t) = 2x(t) \Rightarrow \text{time varying} + \text{linear}$

Laplace Transforms

defn: $F(s) = \int_0^\infty f(t) e^{-st} dt$

$$\mathcal{L}\{f'(t)\} = sF(s) - f(0)$$

$$\mathcal{L}\{f''(t)\} = s^2 F(s) - sf'(0) - f(0)$$

$$\mathcal{L}\{f^{(n)}(t)\} = s^n F(s) - s^{n-1}f^{(n-1)}(0) - s^{n-2}f^{(n-2)}(0) \dots - sf^{(n-1)}(0) - f^{(n-1)}(0)$$

Laplace Transform Table

Continuous time

Differential Equations

$$y^{-1} \left(\begin{array}{l} \text{Impulse Response} \\ \text{Transfer Function} \end{array} \right) y$$

Example 2.2 Show that the Laplace transform is a linear operator

$$\mathcal{L}\{af(t)\} = \int_0^\infty af(t)e^{-st} dt = a \int_0^\infty f(t)e^{-st} dt = a \mathcal{L}\{f(t)\} \quad \checkmark \text{homogeneity holds}$$

$$\mathcal{L}\{f_1(t) + f_2(t)\} = \int_0^\infty (f_1(t) + f_2(t))e^{-st} dt = \int_0^\infty f_1(t)e^{-st} dt + \int_0^\infty f_2(t)e^{-st} dt =$$

$$\mathcal{L}\{f_1(t)\} + \mathcal{L}\{f_2(t)\} \quad \checkmark \text{superposition holds}$$

Why do we care? → Can be useful when solving ODEs

Example 2.3 Suppose we have the following ODE: $\ddot{x}(t) + 3\dot{x}(t) + 2x(t) = f(t)$
Suppose we are given an input $f(t)$ and zero initial conditions. Find $x(t)$.

⇒ Use Laplace Transform

$$\mathcal{L}\{\ddot{x}(t) + 3\dot{x}(t) + 2x(t) = f(t)\} \Rightarrow s^2X(s) + 3sX(s) + 2X(s) = F(s)$$

$$\Rightarrow X(s) = \frac{1}{s^2 + 3s + 2} F(s)$$

↓ output ↓ transfer function ↓ input

★ can find TF by taking Laplace transform of ODE ★

⇒ $f(t) \rightarrow \boxed{\frac{1}{s^2 + 3s + 2}} \rightarrow x(t)$

Suppose we are given $f(t) = \mathcal{U}(t) \rightarrow \text{unit step } \begin{cases} 1, & t \geq 0 \\ 0, & t < 0 \end{cases}$

⇒ From Laplace Transform table $F(s) = \frac{1}{s}$

$$X(s) = \frac{1}{(s^2 + 3s + 2)} \cdot \frac{1}{s} = \frac{A}{s} + \frac{B}{s+1} + \frac{C}{s+2}$$

⇒ use partial fraction decomposition

↳ multiply both sides by s and evaluate @ $s=0 \Rightarrow A = \frac{1}{2}$

↳ multiply both sides by $s+1$ and evaluate @ $s=-1 \Rightarrow B = -1$

↳ multiply both sides by $s+2$ and evaluate @ $s=-2 \Rightarrow C = \frac{1}{2}$

$$X(s) = \frac{1/2}{s} + \frac{-1}{s+1} + \frac{1/2}{s+2}$$

⇒ take inverse Laplace transform

$$x(t) = \mathcal{L}^{-1}\left\{\frac{1/2}{s} + \frac{-1}{s+1} + \frac{1/2}{s+2}\right\} = \frac{1}{2} - e^{-t} + \frac{1}{2}e^{-2t}$$

Example 2.4 Suppose we are given the impulse response of a system is $y(t) = t^2 + e^{2t} + 1, t \geq 0$. Find the transfer function of the system.

↗ System TF

$$Y(s) = G(s)U(s) \quad \text{if } u(t) = \delta(t) \text{ then } u(s) = \mathcal{L}\{\delta(t)\} = 1$$

↙ output ↘ input ↙ impulse

then $Y(s) = G(s) \cdot 1$. So how do we find $G(s)$? Find $Y(s)$ by taking Laplace transform of $y(t)$

$$G(s) = Y(s) = \mathcal{L}\{y(t)\} = \mathcal{L}\{t^2 + e^{2t} + 1\} = \frac{2}{s^3} + \frac{1}{s-2} + \frac{1}{s} = \frac{2s^3 - 2s^2 + 2s - 4}{s^3(s-2)}$$

Impulse response / convolution

let $u(t)$ describe the input signal

let $g(t)$ describe the impulse response of the system

let $y(t)$ describe the output

then $y(t) = (g * u)(t)$ ← convolution yucky

$$= \int_0^t g(t) u(t - \tau) d\tau$$

⇒ given the impulse response of a system, to find the output we can either

Use the $\mathcal{L}\{\}$ to
find TF and find
 $Y(s) = G(s)U(s)$ and
then take $\mathcal{L}^{-1}\{\}$
to find $y(t)$

convolution : (

(I just don't like integrals
unless it's e^x)

Example 2.5 Suppose the impulse response of the system is given by $g(t) = \mathcal{L}^{-1}\{G(s)\} = e^{2t}$. Suppose $u(t) = \mathbb{I}(t)$. Find an expression for $y(t)$

⇒ use convolution

$$y(t) = (g * u)(t) = \int_0^t e^{2\tau} \cdot 1 d\tau = \frac{1}{2} e^{2\tau} \Big|_0^t = \frac{1}{2}(e^{2t} - 1)$$

(I'm telling you, e^x is the only good integral out there)